mc_reify/func_eq.v
@@ -216,7 +216,7 @@ match a, b with
 | fassertD, fassertD => true
 | flocalD , flocalD => true 
 | fstatement s1, fstatement s2 => statement_beq s1 s2
-| ftycontext _ _ _ , ftycontext _ _ _  => true (*TODO*)
+| ftycontext _ _ _ _ , ftycontext _ _ _ _  => true (*TODO*)
 | _, _ => false
 end.
 
