mc_reify/reverse_defs.v
@@ -10,87 +10,118 @@ Proof. eapply mk_listspec; reflexivity. Defined.
 Definition sum_int := fold_right Int.add Int.zero.
 Check var_types.
 Definition Delta : tycontext := 
-(PTree.Node
-          (PTree.Node
+mk_tycontext
+             (PTree.Node
+                (PTree.Node PTree.Leaf None
+                   (PTree.Node
+                      (PTree.Node PTree.Leaf None
+                         (PTree.Node
+                            (PTree.Node PTree.Leaf
+                               (Some (tptr t_struct_list, false)) PTree.Leaf)
+                            None PTree.Leaf)) None PTree.Leaf)) None
+                (PTree.Node
+                   (PTree.Node PTree.Leaf None
+                      (PTree.Node
+                         (PTree.Node
+                            (PTree.Node PTree.Leaf
+                               (Some (tptr t_struct_list, true)) PTree.Leaf)
+                            None PTree.Leaf) None PTree.Leaf)) None
+                   (PTree.Node
+                      (PTree.Node PTree.Leaf None
+                         (PTree.Node
+                            (PTree.Node PTree.Leaf
+                               (Some (tptr t_struct_list, false)) PTree.Leaf)
+                            None PTree.Leaf)) None
+                      (PTree.Node
+                         (PTree.Node
+                            (PTree.Node PTree.Leaf
+                               (Some (tptr t_struct_list, false)) PTree.Leaf)
+                            None PTree.Leaf) None PTree.Leaf))))
+             (PTree.empty type) (tptr t_struct_list)
              (PTree.Node
                 (PTree.Node
-                   (PTree.Node PTree.Leaf (Some (tptr t_struct_list, true))
-                      PTree.Leaf) None PTree.Leaf) None PTree.Leaf) None
-             (PTree.Node PTree.Leaf None
-                (PTree.Node PTree.Leaf (Some (tptr t_struct_list, true))
-                   PTree.Leaf))) None
-          (PTree.Node
+                   (PTree.Node PTree.Leaf None
+                      (PTree.Node
+                         (PTree.Node
+                            (PTree.Node PTree.Leaf
+                               (Some (Tarray t_struct_list 3 noattr))
+                               PTree.Leaf) None PTree.Leaf) None
+                         (PTree.Node
+                            (PTree.Node PTree.Leaf
+                               (Some
+                                  (Tfunction
+                                     (Tcons (tptr t_struct_list) Tnil)
+                                     (tptr t_struct_list) cc_default))
+                               PTree.Leaf) None PTree.Leaf))) None
+                   (PTree.Node PTree.Leaf None
+                      (PTree.Node PTree.Leaf None
+                         (PTree.Node
+                            (PTree.Node PTree.Leaf
+                               (Some (Tfunction Tnil tint cc_default))
+                               PTree.Leaf) None PTree.Leaf)))) None
+                (PTree.Node
+                   (PTree.Node
+                      (PTree.Node PTree.Leaf None
+                         (PTree.Node
+                            (PTree.Node PTree.Leaf
+                               (Some
+                                  (Tfunction
+                                     (Tcons (tptr t_struct_list) Tnil) tint
+                                     cc_default)) PTree.Leaf) None PTree.Leaf))
+                      None PTree.Leaf) None PTree.Leaf))
              (PTree.Node
                 (PTree.Node
-                   (PTree.Node PTree.Leaf (Some (tint, false)) PTree.Leaf)
-                   None PTree.Leaf) None PTree.Leaf) None
-             (PTree.Node PTree.Leaf None
-                (PTree.Node PTree.Leaf (Some (tint, true)) PTree.Leaf))),
-       PTree.empty type, tint,
-       PTree.Node
-         (PTree.Node
-            (PTree.Node
-               (PTree.Node PTree.Leaf
-                  (Some
-                     (Global_func
-                        (WITH _ : unit PRE  [(1%positive, tptr tvoid),
-                         (2%positive, tptr tvoid), 
-                         (3%positive, tuint), (4%positive, tuint)]
-                         (fun _ : environ => !!False) POST  [tvoid]
-                         (fun _ : environ => !!False)))) PTree.Leaf) None
-               PTree.Leaf) None
-            (PTree.Node
-               (PTree.Node
-                  (PTree.Node PTree.Leaf
-                     (Some
-                        (Global_func
-                           (WITH x : share * list int PRE 
-                            [(_p, tptr t_struct_list)]
-                            (let (sh0, contents0) := x in
-                             `(lseg LS sh0 (map Vint contents0)) 
-                               (eval_id _p) `nullval) POST  [tint]
-                            (let (_, contents0) := x in
-                             local (`(eq (Vint (sum_int contents0))) retval)))))
-                     PTree.Leaf) None PTree.Leaf) None PTree.Leaf)) None
-         (PTree.Node
-            (PTree.Node
-               (PTree.Node PTree.Leaf
-                  (Some
-                     (Global_func
-                        (WITH _ : unit PRE  [(1%positive, tptr tschar),
-                         (2%positive, tint)](fun _ : environ => !!False)
-                         POST  [tint](fun _ : environ => !!False))))
-                  PTree.Leaf) None
-               (PTree.Node
-                  (PTree.Node PTree.Leaf
-                     (Some
-                        (Global_func
-                           (WITH x : share * list val PRE 
-                            [(_p, tptr t_struct_list)]
-                            (let (sh0, contents0) := x in
-                             fun x0 : environ =>
-                             !!writable_share sh0 &&
-                             `(lseg LS sh0 contents0) 
-                               (eval_id _p) `nullval x0) POST 
-                            [tptr t_struct_list]
-                            (let (sh0, contents0) := x in
-                             `(lseg LS sh0 (rev contents0)) retval `nullval))))
-                     PTree.Leaf)
-                  (Some (Global_var (Tarray t_struct_list 3 noattr)))
-                  PTree.Leaf)) None
-            (PTree.Node PTree.Leaf
-               (Some
-                  (Global_func
-                     (WITH _ : unit PRE  [(1%positive, tdouble)]
-                      (fun _ : environ => !!False) POST  [tdouble]
-                      (fun _ : environ => !!False))))
-               (PTree.Node
-                  (PTree.Node PTree.Leaf
-                     (Some
-                        (Global_func
-                           (WITH u : unit PRE  []main_pre prog u POST  [tint]
-                            main_post prog u))) PTree.Leaf) None PTree.Leaf)))).
-
+                   (PTree.Node PTree.Leaf None
+                      (PTree.Node PTree.Leaf None
+                         (PTree.Node
+                            (PTree.Node PTree.Leaf
+                               (Some
+                                  (WITH x : share * list val * val PRE 
+                                   [(_p, tptr t_struct_list)]
+                                   (let (p0, p1) := x in
+                                    let (sh0, contents0) := p0 in
+                                    PROP  (writable_share sh0)
+                                    LOCAL  (temp _p p1)
+                                    SEP 
+                                    (`(lseg LS sh0 contents0 p1 nullval)))
+                                   POST  [tptr t_struct_list]
+                                   (let (p0, _) := x in
+                                    let (sh0, contents0) := p0 in
+                                    `(lseg LS sh0 (rev contents0)) retval
+                                      `nullval))) PTree.Leaf) None PTree.Leaf)))
+                   None
+                   (PTree.Node PTree.Leaf None
+                      (PTree.Node PTree.Leaf None
+                         (PTree.Node
+                            (PTree.Node PTree.Leaf
+                               (Some
+                                  (WITH u : unit PRE  []
+                                   main_pre prog u POST  [tint]
+                                   main_post prog u)) PTree.Leaf) None
+                            PTree.Leaf)))) None
+                (PTree.Node
+                   (PTree.Node
+                      (PTree.Node PTree.Leaf None
+                         (PTree.Node
+                            (PTree.Node PTree.Leaf
+                               (Some
+                                  (WITH x : share * list int * val PRE 
+                                   [(_p, tptr t_struct_list)]
+                                   (let (p0, p1) := x in
+                                    let (sh0, contents0) := p0 in
+                                    PROP  ()
+                                    LOCAL  (temp _p p1)
+                                    SEP 
+                                    (`(lseg LS sh0 
+                                         (map Vint contents0) p1 nullval)))
+                                   POST  [tint]
+                                   (let (p0, _) := x in
+                                    let (_, contents0) := p0 in
+                                    local
+                                      (`(eq (Vint (sum_int contents0)))
+                                         retval)))) PTree.Leaf) None
+                            PTree.Leaf)) None PTree.Leaf) None PTree.Leaf)).
+(*
 Definition Delta2 : tycontext :=
 (PTree.Node
            (PTree.Node
@@ -179,4 +210,4 @@ Definition Delta2 : tycontext :=
                          (Global_func
                             (WITH u : unit PRE  []main_pre prog u POST 
                              [tint]main_post prog u))) PTree.Leaf) None
-                   PTree.Leaf)))).*)
+                   PTree.Leaf)))).*)*) 
